src/program_proof/twophase/twophase_proof.v
@@ -1,28 +1,40 @@
+From RecordUpdate Require Import RecordSet.
+From Perennial.algebra Require Import deletable_heap.
 From Perennial.program_proof Require Import proof_prelude.
 From Goose.github_com.mit_pdos.goose_nfsd Require Import twophase.
-From Perennial.program_proof Require Import buftxn_proof.
+From Perennial.program_proof Require Import buftxn.sep_buftxn_proof.
 From Perennial.program_proof Require Import lockmap_proof.
 From Perennial.program_proof Require Import addr.addr_proof buf.buf_proof txn.txn_proof.
 From Perennial.program_proof Require Import wal.abstraction.
 From Perennial.goose_lang.lib Require Import slice.typed_slice.
 From Perennial.Helpers Require Import PropRestore.
 From Perennial.algebra Require Import auth_map.
+From Perennial.program_logic Require Import na_crash_inv.
 
-Section goose_lang.
 Context `{!buftxnG Σ}.
 Context `{!heapG Σ}.
+Definition Nbuftxn := nroot .@ "buftxn".
 
-Definition get_addr_map_blknos {A} (m: gmap addr A) :=
-  dom (gset u64) (gmap_addr_by_block m).
+Definition get_addr_set_blknos (s: gset addr): gset u64 :=
+  set_map addrBlock s.
+
+Definition get_addr_map_blknos {A} (m: gmap addr A): gset u64 :=
+  set_map addrBlock (dom (gset addr) m).
 
 Definition get_disk_blknos (d: disk): gset u64 :=
   set_map (λ x, U64 (x / (block_bytes * 8))) (dom (gset Z) d).
 
+Lemma get_addr_map_blknos_nil {A} :
+  get_addr_map_blknos (∅: gmap addr A) = ∅.
+Proof.
+  set_solver.
+Qed.
+
 Definition addr_wf (dinit: disk) a :=
-  is_Some (dinit !! (addr2flat_z a)) ∧ int.Z (addrOff a) < block_bytes * 8.
+  is_Some (dinit !! (addr2flat_z a)) ∧ int.nat (addrOff a) < block_bytes * 8.
 
 Definition addr_wf' (dinit: disk) a :=
-  (addrBlock a) ∈ get_disk_blknos dinit ∧ int.Z (addrOff a) < block_bytes * 8.
+  (addrBlock a) ∈ get_disk_blknos dinit ∧ int.nat (addrOff a) < block_bytes * 8.
 
 Lemma addr_wf_wf' dinit a:
   addr_wf dinit a → addr_wf' dinit a.
@@ -41,33 +53,102 @@ Proof.
   all: word.
 Qed.
 
-Definition filter_by_key {K A} `{Countable K} P `{!∀ x, Decision (P x)} (m: gmap K A) :=
-  filter (λ x, P x.1) m.
+Section map_filter.
+  Context {K A} (P : K * A → Prop) `{!∀ x, Decision (P x)}.
 
-Lemma filter_by_key_lookup_notin {K A} `{Countable K} P `{!∀ x, Decision (P x)} (m: gmap K A) k :
-  ~ P k → filter_by_key P m !! k = None.
-Proof.
-  intros Hnotin.
-  apply map_filter_lookup_None_2.
-  right.
-  intros x Hacc.
-  auto.
-Qed.
+  Lemma map_filter_always_false `{FinMap K M} (m: M A) :
+    (∀ k x, m !! k = Some x → ¬ P (k, x)) →
+    filter P m = ∅.
+  Proof.
+    intros HP.
+    apply map_empty.
+    intros k.
+    destruct (filter P m !! k) eqn:Hfilter_acc.
+    2: reflexivity.
+    pose proof (map_filter_lookup_Some_1_1 _ _ _ _ Hfilter_acc) as Hacc.
+    apply HP in Hacc.
+    apply map_filter_lookup_Some_1_2 in Hfilter_acc.
+    contradiction.
+  Qed.
 
-Lemma filter_by_key_lookup_in {K A} `{Countable K} P `{!∀ x, Decision (P x)} (m: gmap K A) k :
-  P k → filter_by_key P m !! k = m !! k.
-Proof.
-  intros Hin.
-  destruct (m !! k) as [x|x] eqn:Hlookup.
-  2: {
+  Lemma map_filter_always_true `{FinMap K M} (m: M A) :
+    (∀ k x, m !! k = Some x → P (k, x)) →
+    filter P m = m.
+  Proof.
+    intros HP.
+    apply map_eq.
+    intros k.
+    destruct (m !! k) as [v|] eqn:Hacc.
+    2: apply map_filter_lookup_None_2; intuition.
+    apply map_filter_lookup_Some_2; intuition.
+  Qed.
+
+  Lemma map_filter_Forall_false `{FinMap K M} (m: M A) :
+    map_Forall (λ k x, ¬ P (k, x)) m →
+    filter P m = ∅.
+  Proof.
+    eapply map_filter_always_false.
+  Qed.
+End map_filter.
+
+Definition filter_by_key `{FinMap K M} (Pk: K → Prop) `{!∀ k, Decision (Pk k)} {A} (m: M A) :=
+  filter (λ x, Pk x.1) m.
+
+Section map_filter_by_key.
+  Context `{FinMap K M}.
+  Implicit Types (Pk: K → Prop).
+  Context `{!∀ k, Decision (Pk k)}.
+  Context {A} (m: M A).
+
+  Lemma filter_by_key_lookup_notin k :
+    ¬ Pk k → filter_by_key Pk m !! k = None.
+  Proof.
+    intros Hnotin.
     apply map_filter_lookup_None_2.
+    right.
+    intros x Hacc.
     auto.
-  }
-  apply (map_filter_lookup_Some_2 _ _ _ _ Hlookup).
-  auto.
-Qed.
+  Qed.
 
-Lemma filter_by_key_or {K A} `{Countable K} P1 P2 `{!∀ x, Decision (P1 x)} `{!∀ x, Decision (P2 x)} (m: gmap K A) :
+  Lemma filter_by_key_lookup_in k :
+    Pk k → filter_by_key Pk m !! k = m !! k.
+  Proof.
+    intros Hin.
+    destruct (m !! k) as [x|] eqn:Hlookup.
+    2: {
+      apply map_filter_lookup_None_2.
+      auto.
+    }
+    apply (map_filter_lookup_Some_2 _ _ _ _ Hlookup).
+    auto.
+  Qed.
+
+  Lemma filter_by_key_Forall_false :
+    map_Forall (λ k _, ¬ Pk k) m →
+    filter_by_key Pk m = ∅.
+  Proof.
+    intros HForall.
+    eapply map_filter_always_false.
+    1: assumption.
+    intros k x Hacc.
+    apply (map_Forall_lookup_1 _ _ k x HForall) in Hacc.
+    assumption.
+  Qed.
+
+  Lemma filter_by_key_Forall_true :
+    map_Forall (λ k _, Pk k) m →
+    filter_by_key Pk m = m.
+  Proof.
+    intros HForall.
+    eapply map_filter_always_true.
+    1: assumption.
+    intros k x Hacc.
+    apply (map_Forall_lookup_1 _ _ k x HForall) in Hacc.
+    assumption.
+  Qed.
+End map_filter_by_key.
+
+Lemma filter_by_key_union_or {K A} `{Countable K} P1 P2 `{!∀ x, Decision (P1 x)} `{!∀ x, Decision (P2 x)} (m: gmap K A):
   filter_by_key (λ k, P1 k ∨ P2 k) m =
     filter_by_key P1 m ∪ filter_by_key P2 m.
 Proof.
@@ -89,39 +170,133 @@ Proof.
   destruct (decide (P1 k)) as [Hin1|Hnotin1].
   2: {
     rewrite lookup_union_r.
-    2: apply (filter_by_key_lookup_notin _ _ _ Hnotin1).
+    2: apply (filter_by_key_lookup_notin _ _ Hnotin1).
     apply filter_by_key_lookup_in.
     set_solver.
   }
-  destruct (m !! k) as [x|x] eqn:Hlookup.
+  destruct (m !! k) as [x|] eqn:Hlookup.
   2: {
     apply (iffRL (lookup_union_None _ _ _)).
     split; apply map_filter_lookup_None_2; auto.
   }
   erewrite lookup_union_Some_l; first by auto.
   rewrite -Hlookup.
-  apply (filter_by_key_lookup_in _ _ _ Hin1).
+  apply (filter_by_key_lookup_in _ _ Hin1).
+Qed.
+
+Lemma set_filter_iff `{FinSet K Ct} `{!LeibnizEquiv Ct} P1 P2 `{!∀ x, Decision (P1 x)} `{!∀ x, Decision (P2 x)} (s: Ct):
+  (∀ x, P1 x ↔ P2 x) → filter P1 s = filter P2 s.
+Proof.
+  intros Hiff.
+  rewrite /filter /set_filter.
+  f_equal.
+  apply list_filter_iff.
+  assumption.
+Qed.
+
+Lemma filter_union_or `{FinSet K Ct} `{!LeibnizEquiv Ct} P1 P2 `{!∀ x, Decision (P1 x)} `{!∀ x, Decision (P2 x)} (s: Ct):
+  filter (λ k, P1 k ∨ P2 k) s =
+    filter P1 s ∪ filter P2 s.
+Proof.
+  apply set_eq.
+  intros x.
+  split.
+  - intros Hin.
+    apply elem_of_filter in Hin.
+    apply elem_of_union.
+    destruct Hin as ([HP1|HP2]&Hin).
+    + left.
+      apply elem_of_filter.
+      intuition.
+    + right.
+      apply elem_of_filter.
+      intuition.
+  - intros Hin.
+    apply elem_of_filter.
+    apply elem_of_union in Hin.
+    destruct Hin as [HP1|HP2].
+    + apply elem_of_filter in HP1.
+      intuition.
+    + apply elem_of_filter in HP2.
+      intuition.
+Qed.
+
+Lemma map_subseteq_alt {K A} `{Countable K} `{FinMap K M} (m1 m2: M A) :
+  m1 ⊆ m2 ↔
+  (∀ k v, m1 !! k = Some v → m2 !! k = Some v).
+Proof.
+  rewrite /subseteq /map_subseteq /map_included
+    /map_relation /option_relation.
+  split.
+  - intros Hsubseteq k v.
+    specialize (Hsubseteq k).
+    destruct (m1 !! k) as [v1|].
+    2: intros Hc; inversion Hc.
+    intros Hv1.
+    inversion Hv1.
+    subst v1.
+    destruct (m2 !! k) as [v2|].
+    2: contradiction.
+    subst v2.
+    reflexivity.
+  - intros Halt k.
+    specialize (Halt k).
+    destruct (m1 !! k) as [v1|].
+    2: destruct (m2 !! k); trivial.
+    rewrite (Halt _ (eq_refl _)).
+    reflexivity.
+Qed.
+
+Lemma set_filter_always_false `{Countable K} (s: gset K) P `{!∀ x, Decision (P x)} :
+  (∀ k, k ∈ s → ¬ P k) →
+  filter P s = ∅.
+Proof.
+  intros HP.
+  apply gset.gset_elem_is_empty.
+  intros k Hin.
+  apply elem_of_filter in Hin.
+  specialize (HP k).
+  intuition.
+Qed.
+
+Definition filter_addr_set_by_blk (s_blk: gset u64) (s: gset addr) :=
+  filter (λ a, addrBlock a ∈ s_blk) s.
+
+Lemma filter_addr_set_by_blk_empty (s: gset addr) :
+  filter_addr_set_by_blk (∅: gset u64) s = ∅.
+Proof.
+  rewrite /filter_addr_set_by_blk.
+  apply set_filter_always_false.
+  intros k _.
+  set_solver.
+Qed.
+
+Lemma filter_addr_set_by_blk_union (s1 s2: gset u64) (s: gset addr) :
+  filter_addr_set_by_blk (s1 ∪ s2) s =
+    filter_addr_set_by_blk s1 s ∪ filter_addr_set_by_blk s2 s.
+Proof.
+  rewrite -filter_union_or.
+  apply set_filter_iff.
+  set_solver.
+Qed.
+
+Lemma filter_addr_set_by_blk_disjoint (s1 s2: gset u64) (s: gset addr) :
+  s1 ## s2 →
+  filter_addr_set_by_blk s1 s ## filter_addr_set_by_blk s2 s.
+Proof.
+  intros Hdisj a Hin1 Hin2.
+  specialize (Hdisj (addrBlock a)).
+  destruct (decide (addrBlock a ∈ s1)) as [Hin|Hnotin].
+  - apply elem_of_filter in Hin2.
+    intuition.
+  - apply elem_of_filter in Hin1.
+    intuition.
 Qed.
 
 Definition filter_addr_map_by_blk {A} (s: gset u64) (m: gmap addr A) :=
   filter_by_key (λ a, addrBlock a ∈ s) m.
 
-Lemma map_filter_always_false {K A M} (P : K * A → Prop) `{!∀ x, Decision (P x)} `{FinMap K M} (m: M A) :
-  (∀ k x, m !! k = Some x → ¬ P (k, x)) →
-  filter P m = ∅.
-Proof.
-  intros HP.
-  apply map_empty.
-  intros k.
-  destruct (filter P m !! k) eqn:Hfilter_acc.
-  2: reflexivity.
-  pose proof (map_filter_lookup_Some_1_1 _ _ _ _ Hfilter_acc) as Hacc.
-  apply HP in Hacc.
-  apply map_filter_lookup_Some_1_2 in Hfilter_acc.
-  contradiction.
-Qed.
-
-Lemma filter_addr_map_by_blk_nil {A} (m: gmap addr A) :
+Lemma filter_addr_map_by_blk_empty {A} (m: gmap addr A) :
   filter_addr_map_by_blk (∅: gset u64) m = ∅.
 Proof.
   eapply map_filter_always_false.
@@ -129,11 +304,19 @@ Proof.
   set_solver.
 Qed.
 
+Lemma filter_addr_map_by_blk_subseteq {A} (s: gset u64) (m: gmap addr A) :
+  filter_addr_map_by_blk s m ⊆ m.
+Proof.
+  apply map_subseteq_alt.
+  intros k v Hacc.
+  apply (map_filter_lookup_Some_1_1 _ _ _ _ Hacc).
+Qed.
+
 Lemma filter_addr_map_by_blk_union {A} (s1 s2: gset u64) (m: gmap addr A) :
   filter_addr_map_by_blk (s1 ∪ s2) m =
     filter_addr_map_by_blk s1 m ∪ filter_addr_map_by_blk s2 m.
 Proof.
-  rewrite -filter_by_key_or.
+  rewrite -filter_by_key_union_or.
   apply map_filter_iff.
   set_solver.
 Qed.
@@ -147,16 +330,69 @@ Proof.
   assumption.
 Qed.
 
+Lemma filter_addr_map_by_blk_lookup_notin {A} (s: gset u64) (m: gmap addr A) a :
+  addrBlock a ∉ s →
+  filter_addr_map_by_blk s m !! a = None.
+Proof.
+  intros Hnotin.
+  apply filter_by_key_lookup_notin.
+  assumption.
+Qed.
+
+Lemma filter_addr_map_by_blk_disjoint {A} (s1 s2: gset u64) (m: gmap addr A) :
+  s1 ## s2 →
+  filter_addr_map_by_blk s1 m ##ₘ filter_addr_map_by_blk s2 m.
+Proof.
+  intros Hdisj.
+  apply map_disjoint_alt.
+  pose proof ((iffLR (elem_of_disjoint _ _)) Hdisj) as Hdisj_alt.
+  intros a.
+  destruct (decide (addrBlock a ∈ s1)) as [Hin|Hnotin].
+  - right.
+    specialize (Hdisj_alt _ Hin).
+    apply filter_addr_map_by_blk_lookup_notin.
+    intuition.
+  - left.
+    apply filter_addr_map_by_blk_lookup_notin.
+    assumption.
+Qed.
+
 Lemma filter_addr_map_by_blk_dom_in {A} (s: gset u64) (m: gmap addr A) a :
   a ∈ dom (gset addr) (filter_addr_map_by_blk s m) →
   is_Some (m !! a) ∧ addrBlock a ∈ s.
 Proof.
   intros Hin.
-  apply map_filter_elem_of_dom in Hin.
+  apply mspec.map_filter_elem_of_dom in Hin.
   destruct Hin as [obj [Hacc Ha]].
   apply mk_is_Some in Hacc.
   simpl in Ha.
   intuition.
+Qed.
+
+Lemma filter_addr_map_by_blk_set_dom {A} (s: gset u64) (m: gmap addr A):
+  dom (gset addr) (filter_addr_map_by_blk s m) =
+  filter_addr_set_by_blk s (dom (gset addr) m).
+Proof.
+  apply dom_filter_L.
+  intros a.
+  split.
+  - intros Hin.
+    destruct ((iffLR (elem_of_filter _ _ _)) Hin)
+      as [Hblk Hdom].
+    apply elem_of_dom in Hdom.
+    destruct Hdom as [v Hdom].
+    eexists _.
+    split; first by eassumption.
+    simpl.
+    assumption.
+  - intros Hspec.
+    destruct Hspec as [v [Hacc Hin]].
+    simpl in Hin.
+    apply elem_of_filter.
+    split; first by assumption.
+    apply elem_of_dom.
+    eexists _.
+    eassumption.
 Qed.
 
 Lemma gmap_addr_by_block_filter_by_blk {A} (s: gset u64) (m: gmap addr A):
@@ -274,114 +510,151 @@ Proof.
   inversion Hy.
 Qed.
 
-Implicit Types γ : @txn_names Σ.
+Implicit Types γ : @buftxn_names Σ.
+Implicit Types dinit : disk.
+Implicit Types objs_dom : gset addr.
+Implicit Types mt_changed : gmap addr versioned_object.
+Implicit Types mt_all : gmap addr object.
+Implicit Types mt_committed : gmap addr object.
+Implicit Types blkno : u64.
+Implicit Types inst : nat.
+Implicit Types γdurable_map : gmap nat gname.
+Implicit Types locked_by_map : gmap u64 (option nat).
 
-Definition ptsto_mapsto γ γa a : iProp Σ := (
-  ∃ (v: object),
-    "Hptsto" ∷ ptsto_mut γa a 1 v ∗
-    "Hmapsto" ∷ mapsto_txn γ a v
-)%I.
+Definition modified := mspec.modified.
+Definition committed := mspec.committed.
 
-Definition linv γ metamap blkno : iProp Σ := (
-  [∗ map] a ↦ γa ∈ filter_addr_map_by_blk {[blkno]} metamap, (
-    ptsto_mapsto γ γa a
-  )
-)%I.
+Definition get_lockset_opt locked_by_map inst_opt :=
+  dom (gset u64) (filter (λ x, x.2 = inst_opt) locked_by_map).
 
-Lemma linv_split γ metamap blkno :
-  "Hlinv" ∷ linv γ metamap blkno -∗
-  ∃ (mt: gmap addr object),
-    (
-      let metamap_blk := filter_addr_map_by_blk {[blkno]} metamap in
-      "Hptstos" ∷ [∗ map] a ↦ γa; v ∈ metamap_blk; mt, (
-        "Hptsto" ∷ ptsto_mut γa a 1 v
-      )
-    )
-      ∗
-    (
-      "Hmapstos" ∷ [∗ map] a ↦ v ∈ mt, (
-        "Hmapsto" ∷ mapsto_txn γ a v
-      )
-    ).
+Definition filter_locked_by locked_by_map mt_all inst_opt :=
+  filter_addr_map_by_blk (get_lockset_opt locked_by_map inst_opt) mt_all.
+
+Lemma filter_locked_by_alt locked_by_map mt_all inst_opt :
+  filter_locked_by locked_by_map mt_all inst_opt =
+  filter_by_key
+    (λ a, locked_by_map !! (addrBlock a) = Some inst_opt)
+    mt_all.
 Proof.
-  iIntros.
-  iNamed.
-  iDestruct (big_sepM_sepM2 with "Hlinv") as (mt) "Hlinv".
-  iDestruct (big_sepM2_sep with "Hlinv") as "[Hptstos Hmapstos]".
-  iDestruct (big_sepM2_sepM_2 with "Hmapstos") as "Hmapstos".
-  iDestruct (big_sepM_mono _ (λ k x, "Hmapsto" ∷ mapsto_txn γ k x)
-    with "Hmapstos") as "Hmapstos".
-  {
-    iIntros (k x _) "Φ".
-    iDestruct "Φ" as (x') "[_ Φ]".
-    iAssumption.
+  apply map_eq.
+  intros a.
+  destruct (decide (locked_by_map !! addrBlock a = Some inst_opt))
+    as [Hacc|Hacc].
+  2: {
+    rewrite filter_by_key_lookup_notin.
+    2: assumption.
+    rewrite filter_addr_map_by_blk_lookup_notin; first by reflexivity.
+    intros Hin.
+    rewrite /get_lockset_opt in Hin.
+    apply elem_of_dom in Hin.
+    destruct Hin as [inst_opt' Hinst_opt'].
+    apply map_filter_lookup_Some in Hinst_opt'.
+    destruct Hinst_opt' as [Hacc' Heq].
+    simpl in Heq.
+    subst inst_opt'.
+    contradiction.
   }
-  iExists _.
-  iFrame.
-Qed.
-
-Definition obj_to_vobj (v: object): versioned_object :=
-  existT (projT1 v) (projT2 v, projT2 v).
-
-Lemma linv_lift E buftxnl mt_buftxn γ dinit anydirty metamap blkno:
-  ↑invN ⊆ E →
-  (
-    "Hbuftxn" ∷ is_buftxn buftxnl mt_buftxn γ dinit anydirty ∗
-    "Hlinv" ∷ linv γ metamap blkno
-  )
-    -∗ |NC={E}=>
-  (
-    ∃ mt_new,
-      "Hbuftxn" ∷ is_buftxn buftxnl ((obj_to_vobj <$> mt_new) ∪ mt_buftxn) γ dinit anydirty ∗
-      "Hptstos" ∷ [∗ map] a ↦ γa; v ∈ filter_addr_map_by_blk {[blkno]} metamap; mt_new, (
-        "Hptsto" ∷ ptsto_mut γa a 1 v
-      )
-  ).
-Proof.
-  simpl.
-  intros Hinv.
-  iIntros "(?&?)".
-  iNamed.
-  iDestruct (linv_split with "Hlinv") as (mt_new) "(?&?)".
-  iNamed.
-  iExists mt_new.
-  rewrite /obj_to_vobj.
-  iDestruct (BufTxn_lift _ _ _ _ _ _ _ Hinv with "[$Hbuftxn $Hmapstos]")
-    as "> Hbuftxn".
-  iFrame.
+  rewrite filter_by_key_lookup_in.
+  2: assumption.
+  rewrite filter_addr_map_by_blk_lookup_in; first by reflexivity.
+  apply elem_of_dom.
+  exists inst_opt.
+  apply map_filter_lookup_Some_2.
+  1: assumption.
   auto.
 Qed.
 
-Definition is_twophase_inner (l : loc) mt_buftxn (locks_held: list u64) γ (dinit: disk) metamap : iProp Σ := (
-  ∃ (buftxnl locksl: loc) acquired_s anydirty ghs,
-    let dinit_blknos := get_disk_blknos dinit in
-    let mt_buftxn_blknos := get_addr_map_blknos mt_buftxn in
-    let metamap_blknos := get_addr_map_blknos metamap in
+(*
+Definition buftxn_durable_mapsto γbuftxn inst_state : iProp Σ :=
+  is_buftxn_durable γbuftxn inst_state.(twophase_inst_γdurable)
+    (λ mapsto,
+      [∗ map] a ↦ obj ∈ inst_state.(twophase_inst_mt_committed),
+        mapsto a obj
+    )%I.
+
+Definition twophase_durable_inv_inner γ mt_all : iProp Σ :=
+  ∃ inst_map locked_by_map,
+    let mt_unused := filter_locked_by locked_by_map mt_all None in
+    "Hinst_map_ctx" ∷ map_ctx γ.(twophase_inst_map_name) 1 inst_map ∗
+    "Hlocked_by_ctx" ∷ map_ctx γ.(twophase_locked_by_map_name) 1 locked_by_map ∗
+    "Hmt_used" ∷ (
+      [∗ map] inst ↦ inst_state ∈ inst_map,
+      (
+        "Hbuftxn_durable" ∷ buftxn_durable_mapsto
+          γ inst_state
+      )
+    ) ∗
+    "Hmt_unused" ∷ (
+      [∗ map] a ↦ obj ∈ mt_unused,
+        durable_mapsto γ a obj
+    ) ∗
+    "%Hmt_committed_map" ∷ ⌜map_Forall (λ inst inst_state,
+      inst_state.(twophase_inst_mt_committed) =
+      filter_locked_by locked_by_map mt_all (Some inst)
+    ) inst_map⌝ ∗
+    "%Hlocked_by_wf" ∷ ⌜map_Forall (λ _ inst_opt,
+      ∀ inst, (
+        inst_opt = Some inst →
+        is_Some (inst_map !! inst)
+      )
+    ) locked_by_map⌝.
+
+Definition twophase_durable_inv γ obj_dom P `{!∀ mt_all, Timeless (P mt_all)} : iProp Σ :=
+  ∃ mt_all,
+    "%Hmt_all_dom" ∷ ⌜dom (gset addr) mt_all = obj_dom⌝ ∗
+    "Htwophase_durable_inv" ∷ twophase_durable_inv_inner γ mt_all ∗
+    "HP" ∷ P mt_all.
+
+Global Instance twophase_durable_inv_timeless γ obj_dom P `{!∀ mt_all, Timeless (P mt_all)} :
+  Timeless (twophase_durable_inv γ obj_dom P) := _.
+*)
+
+Definition twophase_linv γ objs_dom blkno : iProp Σ :=
+  "Htokens" ∷ [∗ set] a ∈ filter_addr_set_by_blk {[blkno]} objs_dom, (
+    "Htoken" ∷ modify_token γ a
+  ).
+
+Definition is_twophase_locks (l: loc) γ objs_dom (locks_held: list u64) : iProp Σ :=
+  ∃ (locksl: loc) acquired_s ghs,
+    let objs_dom_blknos := get_addr_set_blknos objs_dom in
     let locked_blknos: gset u64 := list_to_set locks_held in
-    let metamap_in_mt := filter_addr_map_by_blk mt_buftxn_blknos metamap in
-    "Htwophase.buftxn" ∷ l ↦[TwoPhase.S :: "buftxn"] #buftxnl ∗
     "Htwophase.locks" ∷ l ↦[TwoPhase.S :: "locks"] #locksl ∗
-    "Htwophase.acquired" ∷ l ↦[TwoPhase.S :: "acquired"] (slice_val acquired_s) ∗
-    "Hbuftxn" ∷ is_buftxn buftxnl mt_buftxn γ dinit anydirty ∗
-    "#Hlocks" ∷ is_lockMap locksl ghs dinit_blknos (linv γ metamap) ∗
+    "Htwophase.acquired" ∷
+      l ↦[TwoPhase.S :: "acquired"] (slice_val acquired_s) ∗
     "Hacquired_s" ∷ is_slice acquired_s uint64T 1 locks_held ∗
     "Hlocked_blknos" ∷ ([∗ set] blkno ∈ locked_blknos,
       "Hlocked" ∷ Locked ghs blkno
     ) ∗
-    "Hptstos" ∷ ([∗ map] a ↦ γa; vo ∈ metamap_in_mt; mt_buftxn, (
-      "Hptsto" ∷ ptsto_mut γa a 1 (committed vo)
-    )) ∗
-    "%Hmt_buftxn_blknos_locked" ∷ ⌜mt_buftxn_blknos ⊆ locked_blknos⌝ ∗
-    "%Hlocked_blknos_wf" ∷ ⌜locked_blknos ⊆ dinit_blknos⌝ ∗
-    "%Hmetamap_blknos_wf" ∷ ⌜metamap_blknos ⊆ dinit_blknos⌝ ∗
-    "%Hlocks_held_NoDup" ∷ ⌜NoDup locks_held⌝
-)%I.
+    "#HlockMap" ∷ is_lockMap locksl ghs objs_dom_blknos
+      (twophase_linv γ objs_dom) ∗
+    "%Hlocks_held_NoDup" ∷ ⌜NoDup locks_held⌝.
 
-Definition is_twophase (l : loc) mt_buftxn γ (dinit: disk) metamap : iProp Σ := (
+Definition is_twophase_buftxn (l: loc) γ γtxn dinit mt_committed : iProp Σ :=
+  ∃ (buftxnl: loc) γdurable,
+    "Htwophase.buftxn" ∷ l ↦[TwoPhase.S :: "buftxn"] #buftxnl ∗
+    "Hbuftxn_mem" ∷ is_buftxn_mem
+      Nbuftxn buftxnl γ dinit γtxn γdurable ∗
+    "Hbuftxn_durable_frag" ∷ map_ctx γdurable (1/2) mt_committed.
+
+Definition twophase_locked_mapstos γ locked_addrs mt_committed : iProp Σ :=
+  "Hunlifted_mapstos" ∷ (
+    [∗ set] a ∈ locked_addrs ∖ dom (gset addr) mt_committed,
+      "Htoken" ∷ modify_token γ a
+  ) ∗
+  "Hlifted_mapstos" ∷ (
+    [∗ map] a ↦ obj ∈ mt_committed,
+      "Hdurable_mapsto" ∷ durable_mapsto γ a obj
+  ).
+
+Definition is_twophase_raw l γ γtxn dinit objs_dom mt_committed : iProp Σ :=
   ∃ locks_held,
-    "%Hlocks_held" ∷ ⌜list_to_set locks_held = get_addr_map_blknos mt_buftxn⌝ ∗
-    "Htwophase" ∷ is_twophase_inner l mt_buftxn locks_held γ dinit metamap
-)%I.
+    let locked_blknos: gset u64 := list_to_set locks_held in
+    let locked_addrs := filter_addr_set_by_blk locked_blknos objs_dom in
+    "Hlocks" ∷ is_twophase_locks l γ objs_dom locks_held ∗
+    "Hbuftxn" ∷ is_twophase_buftxn l γ γtxn dinit mt_committed ∗
+    "Hlocked_mapstos" ∷ twophase_locked_mapstos γ locked_addrs mt_committed ∗
+    "%Hmt_dom" ∷ ⌜dom (gset addr) mt_committed ⊆ locked_addrs⌝
+  .
 
 Ltac wp_start :=
   iIntros (Φ) "Hpre HΦ";
@@ -395,29 +668,42 @@ Ltac wp_start :=
   | _ => idtac
   end.
 
-Lemma get_addr_map_blknos_nil {A} :
-  get_addr_map_blknos (∅: gmap addr A) = ∅.
+Definition set_max `{FinSet nat Ct} (s: Ct) := list_max (elements s).
+
+Lemma set_in_le_max `{FinSet nat Ct} (s: Ct) x:
+  x ∈ s → x ≤ set_max s.
 Proof.
-  set_solver.
+  intros Hin.
+  unshelve (epose proof (
+    (iffLR (list_max_le (elements s) (set_max s))) _
+  ) as Hthm).
+  1: rewrite /set_max; lia.
+  eapply (iffLR (Forall_forall _ _)) in Hthm.
+  2: apply elem_of_elements; eassumption.
+  assumption.
 Qed.
 
-Theorem wp_twophase_Begin (txnl locksl: loc) γ dinit ghs γmap qmap metamap:
+Theorem wp_TwoPhase__Begin_raw (txnl locksl: loc) γ dinit ghs objs_dom :
   {{{
-    "Htxn" ∷ invariant.is_txn txnl γ dinit ∗
-    "#Hlocks" ∷ is_lockMap locksl ghs (get_disk_blknos dinit) (linv γ metamap)
+    let objs_dom_blknos := get_addr_set_blknos objs_dom in
+    "#Htxn" ∷ (
+      invariant.is_txn txnl γ.(buftxn_txn_names) dinit ∗
+      is_txn_system Nbuftxn γ
+    ) ∗
+    "#Hlocks" ∷ is_lockMap locksl ghs objs_dom_blknos (twophase_linv γ objs_dom)
   }}}
     Begin #txnl #locksl
   {{{
-    (l : loc), RET #l;
-    "%Hmetamap_blknos_wf" ∷ ⌜get_addr_map_blknos metamap ⊆ get_disk_blknos dinit⌝ -∗
-    "Hmetamap_ctx" ∷ map_ctx γmap qmap metamap -∗
-    "Htwophase" ∷ is_twophase l ∅ γ dinit metamap
+    (l : loc) γtxn, RET #l;
+      "Htwophase_raw" ∷ is_twophase_raw l γ γtxn dinit objs_dom ∅
   }}}.
 Proof.
+  simpl.
   wp_start.
   wp_call.
-  wp_apply (wp_buftxn_Begin with "Htxn").
-  iIntros (buftxnl) "Hbuftxn".
+  wp_apply (wp_BufTxn__Begin' with "Htxn").
+  iIntros (? ? buftxnl) "(?&?)".
+  iNamed.
   wp_apply (wp_NewSlice _ _ uint64T).
   iIntros (acquired_s) "Hacquired_s".
   wp_apply wp_allocStruct; first by auto.
@@ -426,109 +712,110 @@ Proof.
   wp_apply util_proof.wp_DPrintf.
   wp_pures.
   iApply "HΦ".
-  iDestruct (struct_fields_split with "Hl") as "(Htwophase.buftxn & Htwophase.locks & Htwophase.acquired & %)".
-  iIntros "? ?".
-  iNamed.
+
   iExists [].
-  iSplit; first by rewrite get_addr_map_blknos_nil //=.
-  iExists _, _, _, _, _.
-  rewrite list_to_set_nil get_addr_map_blknos_nil filter_addr_map_by_blk_nil.
-  iFrame "∗ # %".
-  iSplit; first by auto.
-  iSplit; first by auto.
-  iPureIntro.
-  split; first by auto.
-  split; first by set_solver.
-  apply NoDup_nil_2.
+  iDestruct (struct_fields_split with "Hl") as "(?&?&?&_)".
+  iNamed.
+  iSplitL "locks acquired Hacquired_s".
+  {
+    iExists _, _, _.
+    rewrite list_to_set_nil big_sepS_empty.
+    iFrame "∗ #".
+    iPureIntro.
+    apply NoDup_nil_2.
+  }
+  iSplitL.
+  {
+    iExists _, _.
+    iFrame.
+  }
+  rewrite filter_addr_set_by_blk_empty
+    /twophase_locked_mapstos big_sepM_empty
+    dom_empty_L difference_empty_L big_sepS_empty //.
 Qed.
 
-Lemma set_union_empty_r {A} `{Countable A} (s: gset A) :
-  s ∪ ∅ = s.
-Proof.
-  pose proof (iffRL (set_equiv (s ∪ ∅) s)) as equiv_thm.
-  apply leibniz_equiv.
-  apply (iffRL (set_equiv (s ∪ ∅) s)).
-  set_solver.
-Qed.
+Section map_zip.
+  Context {K A B: Type} `{Countable K} (m1: gmap K A) (m2: gmap K B).
 
-Lemma map_zip_fst {K A B} `{Countable K} (m1: gmap K A) (m2: gmap K B) :
-  dom (gset K) m1 = dom (gset K) m2 →
-  fst <$> (map_zip m1 m2) = m1.
-Proof.
-  intros Hdom.
-  apply map_eq.
-  intros k.
-  rewrite lookup_fmap.
-  destruct (m1 !! k) as [x|] eqn:Hacc.
-  2: rewrite (map_zip_lookup_none_1 _ _ _ Hacc) //.
-  pose proof ((iffRL (elem_of_dom _ _)) (mk_is_Some _ _ Hacc)) as Hkin.
-  rewrite Hdom in Hkin.
-  apply elem_of_dom in Hkin.
-  destruct Hkin as [x2 Hx2].
-  rewrite (map_zip_lookup_some _ _ _ _ _ Hacc Hx2).
-  auto.
-Qed.
+  Lemma map_zip_fst :
+    dom (gset K) m1 = dom (gset K) m2 →
+    fst <$> (map_zip m1 m2) = m1.
+  Proof.
+    intros Hdom.
+    apply map_eq.
+    intros k.
+    rewrite lookup_fmap.
+    destruct (m1 !! k) as [x|] eqn:Hacc.
+    2: rewrite (map_zip_lookup_none_1 _ _ _ Hacc) //.
+    pose proof ((iffRL (elem_of_dom _ _)) (mk_is_Some _ _ Hacc)) as Hkin.
+    rewrite Hdom in Hkin.
+    apply elem_of_dom in Hkin.
+    destruct Hkin as [x2 Hx2].
+    rewrite (map_zip_lookup_some _ _ _ _ _ Hacc Hx2).
+    auto.
+  Qed.
 
-Lemma map_zip_snd {K A B} `{Countable K} (m1: gmap K A) (m2: gmap K B) :
-  dom (gset K) m1 = dom (gset K) m2 →
-  snd <$> (map_zip m1 m2) = m2.
-Proof.
-  intros Hdom.
-  apply map_eq.
-  intros k.
-  rewrite lookup_fmap.
-  destruct (m2 !! k) as [x|] eqn:Hacc.
-  2: rewrite (map_zip_lookup_none_2 _ _ _ Hacc) //.
-  pose proof ((iffRL (elem_of_dom _ _)) (mk_is_Some _ _ Hacc)) as Hkin.
-  rewrite -Hdom in Hkin.
-  apply elem_of_dom in Hkin.
-  destruct Hkin as [x1 Hx1].
-  rewrite (map_zip_lookup_some _ _ _ _ _ Hx1 Hacc).
-  auto.
-Qed.
+  Lemma map_zip_snd :
+    dom (gset K) m1 = dom (gset K) m2 →
+    snd <$> (map_zip m1 m2) = m2.
+  Proof.
+    intros Hdom.
+    apply map_eq.
+    intros k.
+    rewrite lookup_fmap.
+    destruct (m2 !! k) as [x|] eqn:Hacc.
+    2: rewrite (map_zip_lookup_none_2 _ _ _ Hacc) //.
+    pose proof ((iffRL (elem_of_dom _ _)) (mk_is_Some _ _ Hacc)) as Hkin.
+    rewrite -Hdom in Hkin.
+    apply elem_of_dom in Hkin.
+    destruct Hkin as [x1 Hx1].
+    rewrite (map_zip_lookup_some _ _ _ _ _ Hx1 Hacc).
+    auto.
+  Qed.
 
-Lemma map_zip_lookup_some' {K A B} `{Countable K} (m1: gmap K A) (m2: gmap K B) k x1 x2 :
-  map_zip m1 m2 !! k = Some (x1, x2) →
-  m1 !! k = Some x1 ∧ m2 !! k = Some x2.
-Proof.
-  intros Hin.
-  rewrite /map_zip /map_zip_with in Hin.
-  erewrite lookup_merge in Hin.
-  2: rewrite /DiagNone //.
-  destruct (m1 !! k) as [x1'|] eqn:Hx1.
-  2: inversion Hin.
-  destruct (m2 !! k) as [x2'|] eqn:Hx2.
-  2: inversion Hin.
-  inversion Hin.
-  subst.
-  auto.
-Qed.
+  Lemma map_zip_lookup_some' k x1 x2 :
+    map_zip m1 m2 !! k = Some (x1, x2) →
+    m1 !! k = Some x1 ∧ m2 !! k = Some x2.
+  Proof.
+    intros Hin.
+    rewrite /map_zip /map_zip_with in Hin.
+    erewrite lookup_merge in Hin.
+    2: rewrite /DiagNone //.
+    destruct (m1 !! k) as [x1'|] eqn:Hx1.
+    2: inversion Hin.
+    destruct (m2 !! k) as [x2'|] eqn:Hx2.
+    2: inversion Hin.
+    inversion Hin.
+    subst.
+    auto.
+  Qed.
 
-Lemma map_zip_dom {K A B} `{Countable K} (m1: gmap K A) (m2: gmap K B) :
-  dom (gset K) (map_zip m1 m2) = dom (gset K) m1 ∩ dom (gset K) m2.
-Proof.
-  apply set_eq.
-  intros k.
-  split.
-  - intros Hin.
-    apply elem_of_dom in Hin.
-    destruct Hin as (x&Hin).
-    destruct x as (x1&x2).
-    apply map_zip_lookup_some' in Hin.
-    apply elem_of_intersection.
-    destruct Hin as [Hin1 Hin2].
-    split; apply elem_of_dom; eexists _; eassumption.
-  - intros Hin.
-    apply elem_of_intersection in Hin.
-    destruct Hin as [Hin1 Hin2].
-    apply elem_of_dom.
-    apply elem_of_dom in Hin1.
-    apply elem_of_dom in Hin2.
-    destruct Hin1 as [x1 Hin1].
-    destruct Hin2 as [x2 Hin2].
-    eexists _.
-    apply map_zip_lookup_some; eassumption.
-Qed.
+  Lemma map_zip_dom :
+    dom (gset K) (map_zip m1 m2) = dom (gset K) m1 ∩ dom (gset K) m2.
+  Proof.
+    apply set_eq.
+    intros k.
+    split.
+    - intros Hin.
+      apply elem_of_dom in Hin.
+      destruct Hin as (x&Hin).
+      destruct x as (x1&x2).
+      apply map_zip_lookup_some' in Hin.
+      apply elem_of_intersection.
+      destruct Hin as [Hin1 Hin2].
+      split; apply elem_of_dom; eexists _; eassumption.
+    - intros Hin.
+      apply elem_of_intersection in Hin.
+      destruct Hin as [Hin1 Hin2].
+      apply elem_of_dom.
+      apply elem_of_dom in Hin1.
+      apply elem_of_dom in Hin2.
+      destruct Hin1 as [x1 Hin1].
+      destruct Hin2 as [x2 Hin2].
+      eexists _.
+      apply map_zip_lookup_some; eassumption.
+  Qed.
+End map_zip.
 
 Lemma map_zip_same_dom_union {K A B} `{Countable K} (m11 m21: gmap K A) (m12 m22: gmap K B) :
   dom (gset K) m11 = dom (gset K) m12 →
@@ -665,134 +952,75 @@ Proof.
   set_solver.
 Qed.
 
-Theorem wp_twophase__acquireNoCheck (l: loc) mt_buftxn γ dinit metamap (blkno: u64):
+Lemma map_union_least {K A} `{Countable K} `{FinMap K M} (m1 m2 m3: M A) :
+  m1 ⊆ m3 ∧ m2 ⊆ m3 → m1 ∪ m2 ⊆ m3.
+Proof.
+  intros (Hm1&Hm2).
+  apply map_subseteq_union in Hm1.
+  rewrite -Hm1.
+  apply map_union_mono_l.
+  assumption.
+Qed.
+
+Lemma map_filter_mono `{Countable K} `{FinMap K M} {A} (m: M A) P Q `{!∀ x, Decision (P x)} `{!∀ x, Decision (Q x)} :
+  (∀ k v, m !! k = Some v → P (k, v) → Q (k, v)) →
+  filter P m ⊆ filter Q m.
+Proof.
+  intros Hmono.
+  eapply (iffRL (map_subseteq_alt _ _)).
+  intros k v Hfilter_acc.
+  assert (m !! k = Some v) as Hacc by (
+    eapply map_filter_lookup_Some_1_1; eassumption
+  ).
+  apply (map_filter_lookup_Some_2 _ _ _ _ Hacc).
+  apply (Hmono _ _ Hacc).
+  apply (map_filter_lookup_Some_1_2 _ _ _ _ Hfilter_acc).
+Qed.
+
+Lemma set_filter_mono `{FinSet K Ct} (s: Ct) P Q `{!∀ x, Decision (P x)} `{!∀ x, Decision (Q x)} :
+  (∀ k, k ∈ s → P k → Q k) →
+  filter P s ⊆ filter Q s.
+Proof.
+  intros Hmono.
+  intros k HinP.
+  apply elem_of_filter in HinP.
+  apply elem_of_filter.
+  intuition.
+Qed.
+
+Lemma set_disjoint_weaken_l `{FinSet K Ct} (s1 s1' s2: Ct) :
+  s1' ## s2 → s1 ⊆ s1' → s1 ## s2.
+Proof.
+  set_solver.
+Qed.
+
+Lemma subseteq_trans `{FinSet K Ct} (s1 s2 s3: Ct) :
+  s1 ⊆ s2 → s2 ⊆ s3 → s1 ⊆ s3.
+Proof.
+  set_solver.
+Qed.
+
+Theorem wp_TwoPhase__acquireNoCheck (l: loc) γ (blkno: u64) objs_dom locks_held:
+  blkno ∈ get_addr_set_blknos objs_dom →
+  blkno ∉ locks_held →
   {{{
-    "Htwophase" ∷ is_twophase l mt_buftxn γ dinit metamap ∗
-    "%Hblkno_wf" ∷ ⌜blkno ∈ get_disk_blknos dinit⌝ ∗
-    "%Hblkno_in_metamap" ∷ ⌜blkno ∈ get_addr_map_blknos metamap⌝ ∗
-    "%Hblkno_not_locked" ∷ ⌜blkno ∉ get_addr_map_blknos mt_buftxn⌝
+    "Hlocks" ∷ is_twophase_locks l γ objs_dom locks_held
   }}}
     TwoPhase__acquireNoCheck #l #blkno
   {{{
     RET #();
-    ∃ mt_buftxn',
-      "%Hmt_buftxn'_blknos" ∷ ⌜
-        get_addr_map_blknos mt_buftxn' =
-        get_addr_map_blknos mt_buftxn ∪ {[blkno]}
-      ⌝ ∗
-      "Htwophase" ∷ is_twophase l mt_buftxn' γ dinit metamap
+    "Hlocks" ∷ is_twophase_locks l γ objs_dom (locks_held ++ [blkno]) ∗
+    "Hlinv" ∷ twophase_linv γ objs_dom blkno
   }}}.
 Proof.
+  intros Hblkno_wf Hblkno_not_locked.
   wp_start.
   wp_call.
-  iNamed "Htwophase".
-  iNamed "Htwophase".
+  iNamed "Hlocks".
   wp_loadField.
-  wp_apply (wp_LockMap__Acquire with "[$Hlocks]").
+  wp_apply (wp_LockMap__Acquire with "[$HlockMap]").
   1: iPureIntro; assumption.
   iIntros "[Hlinv Hlocked]".
-  iNamed "Hlinv".
-
-  iDestruct (linv_lift with "[$Hbuftxn $Hlinv]") as "> Hlinv".
-  1: auto.
-  iDestruct "Hlinv" as (?) "[? Hptstos_new]".
-  iDestruct (from_named with "Hptstos_new") as "Hptstos_new".
-  iNamed.
-  replace ([∗ map] a↦γa;v ∈ _;mt_new, _)%I
-    with ([∗ map] a↦γa;v ∈
-      filter_addr_map_by_blk {[blkno]} metamap;
-      committed <$> (obj_to_vobj <$> mt_new),
-        "Hptsto" ∷ a [[γa]]↦ v
-    )%I.
-  2: {
-    f_equal.
-    rewrite -map_fmap_compose.
-    rewrite (map_fmap_ext _ id).
-    1: rewrite map_fmap_id //.
-    intros _ x _.
-    destruct x.
-    rewrite /obj_to_vobj /committed //=.
-  }
-  rewrite big_sepM2_fmap_r.
-  iDestruct (big_sepM2_dom with "Hptstos") as "%Hptstos_dom".
-  iDestruct (big_sepM2_dom with "Hptstos_new") as "%Hptstos_new_dom".
-  rewrite big_sepM2_to_sepM_zip big_sepM2_to_sepM_zip.
-  assert (mt_buftxn ##ₘ (obj_to_vobj <$> mt_new)) as Hdisj.
-  {
-    apply map_disjoint_dom_2.
-    rewrite -Hptstos_dom -Hptstos_new_dom.
-    apply map_disjoint_dom_1.
-    apply map_disjoint_alt.
-    intros k.
-    destruct (decide (addrBlock k = blkno)) as [Hk_blk|Hk_blk].
-    - left.
-      apply filter_by_key_lookup_notin.
-      rewrite Hk_blk.
-      set_solver.
-    - right.
-      apply filter_by_key_lookup_notin.
-      set_solver.
-  }
-  rewrite (map_union_comm _ _ (map_disjoint_comm _ _ Hdisj)).
-  unshelve (iDestruct ((equiv_entails_sym _ _ (big_sepM_union _ _ _ _)) with "[$Hptstos $Hptstos_new]") as "Hptstos").
-  {
-    apply map_disjoint_dom_2.
-    rewrite map_zip_dom map_zip_dom Hptstos_dom Hptstos_new_dom.
-    rewrite -> subseteq_intersection_1 by set_solver.
-    rewrite -> subseteq_intersection_1 by set_solver.
-    apply map_disjoint_dom_1.
-    apply Hdisj.
-  }
-  rewrite (map_zip_same_dom_union _ _ _ _ Hptstos_dom Hptstos_new_dom).
-  iDestruct (big_sepM_zip_to_sepM2 with "Hptstos") as "Hptstos".
-  1: rewrite dom_union_L dom_union_L Hptstos_dom Hptstos_new_dom //.
-  rewrite -filter_addr_map_by_blk_union /=.
-  assert (
-    get_addr_map_blknos (obj_to_vobj <$> mt_new) = {[blkno]}
-  ) as Hmt_new_blknos.
-  {
-    rewrite /get_addr_map_blknos.
-    eapply set_eq.
-    intros blkno'.
-    split.
-    - intros Hin.
-      apply elem_of_dom in Hin.
-      apply gmap_addr_by_block_lookup_is_Some in Hin.
-      destruct Hin as [off Hin].
-      apply elem_of_dom in Hin.
-      rewrite -Hptstos_new_dom in Hin.
-      apply filter_addr_map_by_blk_dom_in in Hin.
-      destruct Hin as [_ Hin].
-      simpl in Hin.
-      assumption.
-    - intros Hin.
-      apply elem_of_singleton_1 in Hin.
-      subst blkno.
-      rewrite -(gmap_addr_by_block_dom_eq Hptstos_new_dom)
-        gmap_addr_by_block_filter_by_blk.
-      apply map_filter_elem_of_dom.
-      rewrite /get_addr_map_blknos in Hblkno_in_metamap.
-      apply elem_of_dom in Hblkno_in_metamap.
-      destruct Hblkno_in_metamap as [metamap_blk Hmetamap_blk].
-      eexists _.
-      split; first by eassumption.
-      simpl.
-      set_solver.
-  }
-  assert (
-    get_addr_map_blknos (mt_buftxn ∪ (obj_to_vobj <$> mt_new))
-      =
-    list_to_set locks_held ∪ {[blkno]}
-  ) as Hlocked_blknos'.
-  {
-    rewrite /get_addr_map_blknos gmap_addr_by_block_dom_union.
-    f_equal.
-    1: rewrite Hlocks_held //.
-    apply Hmt_new_blknos.
-  }
-  rewrite -Hmt_new_blknos.
-  rewrite -gmap_addr_by_block_dom_union.
-
   wp_loadField.
   wp_apply (wp_SliceAppend (V:=u64) with "[$Hacquired_s]").
   iIntros (acquired_s') "Hacquired_s".
@@ -801,78 +1029,47 @@ Proof.
   iIntros "Htwophase.acquired".
   iApply "HΦ".
 
-  iExists _.
+  iFrame "Hlinv".
+  iExists _, _, _.
+  iFrame "∗ #".
   iSplit.
-  2: {
-    iExists _.
-    iSplit.
-    2: {
-      iExists _, _, _, _, _.
-      iFrame (Hmetamap_blknos_wf) "∗ #".
-      rewrite list_to_set_app_L /= set_union_empty_r.
-      iSplitL "Hlocked_blknos Hlocked".
-      {
-        rewrite set_union_comm big_sepS_insert.
-        1: iFrame.
-        rewrite Hlocks_held.
-        assumption.
-      }
-      iPureIntro.
-      split.
-      {
-        rewrite -Hlocked_blknos'.
-        set_solver.
-      }
-      split.
-      {
-        apply union_least.
-        1: assumption.
-        apply elem_of_subseteq_singleton.
-        assumption.
-      }
-      apply NoDup_app.
-      split; first by assumption.
-      split.
-      2: apply NoDup_singleton.
-      intros blkno' Hin His.
-      apply elem_of_list_singleton in His.
-      subst blkno.
-      apply (iffRL (@elem_of_list_to_set _ (gset u64) _ _ _ _ _ _ _)) in Hin.
-      rewrite Hlocks_held in Hin.
-      contradiction.
-    }
-    iPureIntro.
-    rewrite list_to_set_app_L /= set_union_empty_r.
-    symmetry.
-    apply Hlocked_blknos'.
+  {
+    rewrite list_to_set_app_L
+      (leibniz_equiv _ _ (list_to_set_singleton _)).
+    iApply big_sepS_union.
+    2: iFrame; iApply big_sepS_singleton; iFrame.
+    intros blkno' Hin1 Hin2.
+    apply (iffLR (elem_of_singleton _ _)) in Hin2.
+    subst blkno'.
+    apply elem_of_list_to_set in Hin1.
+    contradiction.
   }
   iPureIntro.
-  rewrite Hlocked_blknos' Hlocks_held //.
+  apply NoDup_app.
+  split; first by assumption.
+  split.
+  2: apply NoDup_singleton.
+  intros blkno' Hin1 Hin2.
+  apply elem_of_list_singleton in Hin2.
+  subst blkno'.
+  contradiction.
 Qed.
 
-Theorem wp_twophase__Acquire (l: loc) mt_buftxn γ dinit metamap (blkno: u64):
+Theorem wp_TwoPhase__isAlreadyAcquired (l: loc) γ objs_dom locks_held blkno :
   {{{
-    "Htwophase" ∷ is_twophase l mt_buftxn γ dinit metamap ∗
-    "%Hblkno_wf" ∷ ⌜blkno ∈ get_disk_blknos dinit⌝ ∗
-    "%Hblkno_in_metamap" ∷ ⌜blkno ∈ get_addr_map_blknos metamap⌝
+    "Hlocks" ∷ is_twophase_locks l γ objs_dom locks_held
   }}}
-    TwoPhase__Acquire #l #blkno
+    TwoPhase__isAlreadyAcquired #l #blkno
   {{{
-    RET #();
-    ∃ mt_buftxn',
-      "%Hmt_buftxn'_blknos" ∷ ⌜
-        get_addr_map_blknos mt_buftxn' =
-        get_addr_map_blknos mt_buftxn ∪ {[blkno]}
-      ⌝ ∗
-      "Htwophase" ∷ is_twophase l mt_buftxn' γ dinit metamap
+    RET #(bool_decide (blkno ∈ locks_held));
+    "Hlocks" ∷ is_twophase_locks l γ objs_dom locks_held
   }}}.
 Proof.
   wp_start.
   wp_call.
   wp_apply wp_ref_to; first by auto.
   iIntros (already_acquired_l) "Halready_acquired_l".
-  iNamed "Htwophase".
-  iNamed "Htwophase".
+  iNamed "Hlocks".
   wp_loadField.
   iDestruct (is_slice_small_read with "Hacquired_s") as "[Hacquired_s Hacquired_s_wrap]".
   wp_apply (wp_forSlicePrefix (λ done todo,
@@ -925,60 +1122,331 @@ Proof.
   iApply "Hacquired_s_wrap" in "Hacquired_s".
   wp_apply (wp_LoadAt with "[$Halready_acquired_l]").
   iIntros "Halready_acquired_l".
+  iApply "HΦ".
+  iExists _, _, _.
+  iFrame "∗ # %".
+Qed.
+
+Theorem wp_TwoPhase__Acquire (l: loc) γ objs_dom locks_held (blkno: u64):
+  blkno ∈ get_addr_set_blknos objs_dom →
+  {{{
+    "Hlocks" ∷ is_twophase_locks l γ objs_dom locks_held
+  }}}
+    TwoPhase__Acquire #l #blkno
+  {{{
+    RET #();
+    if (decide (blkno ∈ locks_held)) then
+      "Hlocks" ∷ is_twophase_locks l γ objs_dom locks_held
+    else (
+      "Hlocks" ∷ is_twophase_locks l γ objs_dom (locks_held ++ [blkno]) ∗
+      "Hlinv" ∷ twophase_linv γ objs_dom blkno
+    )
+  }}}.
+Proof.
+  intros Hwf.
+  wp_start.
+  wp_call.
+  wp_apply (wp_TwoPhase__isAlreadyAcquired with "Hlocks").
+  iNamed 1.
   wp_if_destruct.
   2: {
     iApply "HΦ".
-    iExists mt_buftxn.
-    apply (@elem_of_list_to_set _ (gset u64) _ _ _ _ _) in Heqb.
-    rewrite Hlocks_held in Heqb.
-    iSplit; first by (iPureIntro; set_solver).
-    iExists locks_held.
-    iSplit; first by (iPureIntro; assumption).
-    iExists _, _, _, _, _.
-    iFrame "∗ # %".
+    rewrite (decide_True _ _ Heqb).
+    iFrame.
   }
-  rewrite bool_decide_eq_false_2.
-  2: assumption.
-  wp_apply (wp_twophase__acquireNoCheck with "[
-    Htwophase.buftxn Htwophase.locks Htwophase.acquired
-    Hbuftxn Hlocked_blknos Hptstos Hacquired_s
-  ]").
-  {
-    apply (@not_elem_of_list_to_set _ (gset u64) _ _ _ _ _) in Heqb.
-    rewrite Hlocks_held in Heqb.
-    iFrame (Hblkno_wf Hblkno_in_metamap Heqb).
-    iExists locks_held.
-    iSplit; first by (iPureIntro; assumption).
-    iExists _, _, _, _, _.
-    iFrame "∗ # %".
-  }
-  iIntros "Hpost".
-  iNamed "Hpost".
+  wp_apply (wp_TwoPhase__acquireNoCheck with "Hlocks").
+  1-2: assumption.
+  iNamed 1.
   iApply "HΦ".
-  iExists _.
-  iFrame (Hmt_buftxn'_blknos) "∗".
+  rewrite (decide_False _ _ Heqb).
+  iFrame.
 Qed.
 
-Theorem wp_twophase__Release (l: loc) locked_blknos blkno γ dinit metamap:
+Lemma twophase_locked_mapstos_add γ locked_blknos mt_committed objs_dom blkno :
+  dom (gset addr) mt_committed ⊆
+    filter_addr_set_by_blk locked_blknos objs_dom →
+  blkno ∉ locked_blknos →
+  "Hmapstos" ∷ twophase_locked_mapstos
+    γ (filter_addr_set_by_blk locked_blknos objs_dom) mt_committed -∗
+  "Hlinv" ∷ twophase_linv γ objs_dom blkno -∗
+    "Hmapstos" ∷ twophase_locked_mapstos
+      γ (filter_addr_set_by_blk (locked_blknos ∪ {[blkno]}) objs_dom)
+      mt_committed.
+Proof.
+  iIntros (Hmt_dom Hnew) "??".
+  iNamed.
+  iDestruct "Hmapstos" as "(?&?)".
+  iNamed.
+  iFrame.
+  rewrite filter_addr_set_by_blk_union difference_union_distr_l_L.
+  iApply big_sepS_union.
+  {
+    apply disjoint_difference_l2.
+    apply disjoint_difference_r2.
+    apply filter_addr_set_by_blk_disjoint.
+    apply disjoint_singleton_r.
+    assumption.
+  }
+  iFrame.
+  rewrite difference_disjoint_L.
+  2: {
+    apply disjoint_sym.
+    eapply set_disjoint_weaken_l; last by eassumption.
+    apply filter_addr_set_by_blk_disjoint.
+    apply disjoint_singleton_r.
+    assumption.
+  }
+  iFrame.
+Qed.
+
+Theorem wp_TwoPhase__Acquire_merge (l: loc) γ objs_dom locks_held mt_committed (blkno: u64):
+  dom (gset addr) mt_committed ⊆
+    filter_addr_set_by_blk (list_to_set locks_held) objs_dom →
+  blkno ∈ get_addr_set_blknos objs_dom →
   {{{
-    "Htwophase" ∷ is_twophase_inner l ∅ (locked_blknos ++ [blkno]) γ dinit metamap ∗
-    "Hlinv" ∷ linv γ metamap blkno
+    "Hlocks" ∷ is_twophase_locks l γ objs_dom locks_held ∗
+    "Hmapstos" ∷ twophase_locked_mapstos
+      γ (filter_addr_set_by_blk
+      (list_to_set locks_held) objs_dom) mt_committed
+  }}}
+    TwoPhase__Acquire #l #blkno
+  {{{
+    RET #();
+    let locks_held' := (
+      if (decide (blkno ∈ locks_held)) then
+        locks_held
+      else
+        locks_held ++ [blkno]
+    ) in
+    "Hlocks" ∷ is_twophase_locks l γ objs_dom locks_held' ∗
+    "Hmapstos" ∷ twophase_locked_mapstos
+      γ (filter_addr_set_by_blk
+      (list_to_set locks_held') objs_dom) mt_committed
+  }}}.
+Proof.
+  iIntros (Hmt_dom Hwf).
+  wp_start.
+  wp_apply (wp_TwoPhase__Acquire with "Hlocks");
+    first by assumption.
+  destruct (decide (blkno ∈ locks_held)) as [Hlocked|Hnot_locked].
+  {
+    iNamed 1.
+    iApply "HΦ".
+    iFrame.
+  }
+  iNamed 1.
+
+  iApply "HΦ".
+  iDestruct (twophase_locked_mapstos_add with "Hmapstos Hlinv")
+    as "?"; [by assumption|apply not_elem_of_list_to_set; assumption|].
+  iNamed.
+  rewrite list_to_set_app_L
+    (leibniz_equiv _ _ (list_to_set_singleton _)).
+  iFrame.
+Qed.
+
+Lemma is_twophase_buftxn_not_in_map l γ γtxn dinit mt_committed a obj :
+  "Hbuftxn" ∷ is_twophase_buftxn l γ γtxn dinit mt_committed -∗
+  "Hold_vals" ∷ (
+    [∗ map] a ↦ obj ∈ mt_committed,
+      "Hdurable_mapsto" ∷ durable_mapsto γ a obj
+  ) -∗
+  "Hdurable_mapsto" ∷ durable_mapsto γ a obj -∗
+  ⌜mt_committed !! a = None⌝.
+Proof.
+  iIntros "???".
+  iNamed.
+  iNamed "Hbuftxn".
+  iNamed "Hbuftxn_mem".
+  iDestruct (map_ctx_agree with "Hbuftxn_durable_frag Hdurable") as %<-.
+  iApply (
+    is_buftxn_durable_not_in_map with
+    "Hdurable_mapsto [Hbuftxn_durable_frag Hold_vals] Hdurable"
+  ).
+  iExists _.
+  iFrame.
+  iModIntro.
+  iIntros (?) "Hmapstos".
+  trivial.
+Qed.
+
+Theorem twophase_lift l γ dinit γtxn locked_addrs mt_committed a obj :
+  a ∈ locked_addrs →
+  "Hbuftxn" ∷ is_twophase_buftxn l γ γtxn dinit mt_committed -∗
+  "Hmapstos" ∷ twophase_locked_mapstos γ locked_addrs mt_committed -∗
+  "Hdurable_mapsto" ∷ durable_mapsto γ a obj
+  -∗ |NC={⊤}=>
+  "Hbuftxn" ∷ is_twophase_buftxn
+    l γ γtxn dinit (<[a:=obj]>mt_committed) ∗
+  "Hmapstos" ∷ twophase_locked_mapstos
+    γ locked_addrs (<[a:=obj]>mt_committed) ∗
+  "Hbuftxn_maps_to" ∷ buftxn_maps_to γtxn a obj.
+Proof.
+  iIntros (Hlocked) "???".
+  iNamed.
+  iNamed "Hmapstos".
+  iDestruct (
+    is_twophase_buftxn_not_in_map with
+    "Hbuftxn Hlifted_mapstos Hdurable_mapsto"
+  ) as "%Hnotin".
+  iNamed "Hbuftxn".
+  apply not_elem_of_dom in Hnotin.
+  iDestruct (big_sepS_delete _ _ a with "Hunlifted_mapstos")
+    as "[? Hunlifted_mapstos]";
+    first by set_solver.
+  iNamed.
+  iMod (lift_into_txn' with "
+    Hbuftxn_mem Hbuftxn_durable_frag Hlifted_mapstos
+    [Hdurable_mapsto Htoken]
+  ") as "(?&?&?&?&?)".
+  1-3: solve_ndisj.
+  1: iFrame.
+  iNamed.
+  iModIntro.
+  iFrame "Hbuftxn_maps_to".
+  iSplitL "Htwophase.buftxn Hbuftxn_mem Hdurable_frag";
+   first by (iExists _, _; iFrame).
+ iFrame.
+ rewrite dom_insert_L set_union_comm -difference_difference_L.
+ iFrame.
+Qed.
+
+Theorem twophase_lift_if_needed l γ dinit γtxn locked_addrs mt_committed a obj :
+  a ∈ locked_addrs →
+  "Hbuftxn" ∷ is_twophase_buftxn l γ γtxn dinit mt_committed -∗
+  "Hmapstos" ∷ twophase_locked_mapstos γ locked_addrs mt_committed -∗
+  "Hmapsto" ∷ (
+    match mt_committed !! a with
+    | Some _ => buftxn_maps_to γtxn a obj
+    | None => durable_mapsto γ a obj
+    end
+  )
+  -∗ |NC={⊤}=>
+  let mt_committed' :=
+    match mt_committed !! a with
+    | Some _ => mt_committed
+    | None => <[a:=obj]>mt_committed
+    end
+  in
+  "Hbuftxn" ∷ is_twophase_buftxn l γ γtxn dinit mt_committed' ∗
+  "Hmapstos" ∷ twophase_locked_mapstos γ locked_addrs mt_committed' ∗
+  "Hbuftxn_maps_to" ∷ buftxn_maps_to γtxn a obj.
+Proof.
+  iIntros (Hlocked) "???".
+  iNamed.
+  destruct (mt_committed !! a) as [old_obj|] eqn:Hlookup_old;
+    first by (iModIntro; iFrame).
+  iMod (twophase_lift with "Hbuftxn Hmapstos Hmapsto") as "(?&?&?)";
+    first by assumption.
+  iNamed.
+  iModIntro.
+  iFrame.
+Qed.
+
+Theorem wp_TwoPhase__Acquire_lift (l: loc) γ γtxn dinit objs_dom mt_committed a obj:
+  a ∈ objs_dom →
+  {{{
+    "Htwophase" ∷ is_twophase_raw l γ γtxn dinit objs_dom mt_committed ∗
+    "Hmapsto" ∷ (
+      match mt_committed !! a with
+      | Some _ => buftxn_maps_to γtxn a obj
+      | None => durable_mapsto γ a obj
+      end
+    )
+  }}}
+    TwoPhase__Acquire #l #(addrBlock a)
+  {{{
+    RET #();
+    let mt_committed' :=
+      match mt_committed !! a with
+      | Some _ => mt_committed
+      | None => <[a:=obj]>mt_committed
+      end
+    in
+    "Htwophase" ∷ is_twophase_raw l γ γtxn dinit objs_dom mt_committed' ∗
+    "Hmapsto" ∷ buftxn_maps_to γtxn a obj
+  }}}.
+Proof.
+  iIntros (Hwf).
+  wp_start.
+  iNamed "Htwophase".
+  iApply wp_ncfupd.
+  wp_apply (wp_TwoPhase__Acquire_merge with "[$Hlocks $Hlocked_mapstos]");
+    [assumption|apply elem_of_map_2; assumption|].
+  iNamed 1.
+  iMod (twophase_lift_if_needed with "Hbuftxn Hmapstos Hmapsto")
+    as "(?&?&?)".
+  {
+    apply elem_of_filter.
+    split; last by assumption.
+    apply elem_of_list_to_set.
+    destruct (decide (addrBlock a ∈ locks_held)); first by assumption.
+    apply elem_of_app.
+    right.
+    apply elem_of_list_singleton.
+    reflexivity.
+  }
+  iNamed.
+  iModIntro.
+  iApply "HΦ".
+  iFrame "Hbuftxn_maps_to".
+  iExists _.
+  iFrame.
+  iPureIntro.
+  destruct (mt_committed !! a) as [old_obj|] eqn:Hlookup_old.
+  {
+    apply mk_is_Some in Hlookup_old.
+    rewrite decide_True; first by assumption.
+    apply elem_of_dom in Hlookup_old.
+    specialize (Hmt_dom a Hlookup_old).
+    apply elem_of_filter in Hmt_dom.
+    destruct Hmt_dom as [Hlocked Hwf_strong].
+    apply elem_of_list_to_set in Hlocked.
+    apply Hlocked.
+  }
+  rewrite dom_insert.
+  destruct (decide (addrBlock a ∈ locks_held)) as [Hlocked|Hnot_locked].
+  {
+    apply union_least; last by assumption.
+    apply elem_of_subseteq_singleton.
+    apply elem_of_filter.
+    split; last by assumption.
+    apply elem_of_list_to_set.
+    assumption.
+  }
+  rewrite list_to_set_app_L
+    (leibniz_equiv _ _ (list_to_set_singleton _))
+    filter_addr_set_by_blk_union
+    union_comm.
+  apply union_mono; first by assumption.
+  apply elem_of_subseteq_singleton.
+  apply elem_of_filter.
+  split; last by assumption.
+  set_solver.
+Qed.
+
+Theorem wp_TwoPhase__Release (l: loc) γ locks_held blkno objs_dom :
+  {{{
+    "Hlocks" ∷ is_twophase_locks
+      l γ objs_dom (locks_held ++ [blkno]) ∗
+    "Hlinv" ∷ twophase_linv γ objs_dom blkno
   }}}
     TwoPhase__Release #l
   {{{
     RET #();
-    is_twophase_inner l ∅ locked_blknos γ dinit metamap
+    "Hlocks" ∷ is_twophase_locks l γ objs_dom locks_held
   }}}.
 Proof.
   wp_start.
   wp_call.
-  iNamed "Htwophase".
+  iNamed "Hlocks".
   wp_loadField.
   wp_apply wp_slice_len.
   wp_loadField.
   iDestruct (is_slice_small_read with "Hacquired_s") as "[Hacquired_s Hacquired_s_wrap]".
   iDestruct (is_slice_small_sz with "Hacquired_s") as "%Hacquired_s_sz".
-  assert ((locked_blknos ++ [blkno]) !! (length locked_blknos) = Some blkno) as Hlocked_blknos_acc.
+  assert ((locks_held ++ [blkno]) !! (length locks_held) = Some blkno)
+    as Hlocked_blknos_acc.
   {
     rewrite -> lookup_app_r by lia.
     rewrite Nat.sub_diag //.
@@ -993,140 +1461,451 @@ Proof.
     apply Hlocked_blknos_acc.
   }
   iIntros "Hacquired_s".
+  iApply "Hacquired_s_wrap" in "Hacquired_s".
   wp_loadField.
   rewrite list_to_set_app_L.
-  iDestruct (big_sepS_union with "Hlocked_blknos") as "[Hlocked_blknos Hlocked]".
+  iDestruct (big_sepS_union with "Hlocked_blknos")
+    as "[Hlocked_blknos Hlocked]".
   {
-    (* this can be a lemma *)
     apply NoDup_app in Hlocks_held_NoDup.
     destruct Hlocks_held_NoDup as (_ & Hdisj & _).
-    apply elem_of_disjoint.
-    intros x.
-    intros Hin1 Hin2.
-    apply elem_of_list_to_set in Hin1.
-    apply elem_of_list_to_set in Hin2.
-    apply Hdisj in Hin1.
-    contradiction.
+    set_solver.
   }
-  rewrite /= set_union_empty_r big_sepS_singleton.
-  wp_apply (wp_LockMap__Release with "[$Hlocks $Hlocked $Hlinv]").
+  rewrite /= union_empty_r_L big_sepS_singleton.
+  iNamed "Hlocked".
+  wp_apply (wp_LockMap__Release with "[$HlockMap $Hlocked $Hlinv]").
   wp_loadField.
   wp_apply (wp_SliceTake uint64T).
   1: word.
   wp_apply (wp_storeField with "Htwophase.acquired").
   1: rewrite /field_ty /=; val_ty.
   iIntros "Htwophase.acquired".
+
   iApply "HΦ".
-  iExists _, _, _, _, _.
-  iApply "Hacquired_s_wrap" in "Hacquired_s".
+  iExists _, _, _.
   iFrame "∗ #".
-  iSplitL "Hacquired_s".
-  {
-    iApply (is_slice_take_cap _ _ _ (word.sub acquired_s.(Slice.sz) 1)) in "Hacquired_s".
-    1: rewrite fmap_length app_length /=; word.
-    replace (int.nat (word.sub _ 1)) with ((int.nat acquired_s.(Slice.sz)) - 1)%nat by word.
-    rewrite -fmap_take -Hacquired_s_sz Nat.add_sub take_app.
-    iFrame.
-  }
-  iPureIntro.
-  rewrite get_addr_map_blknos_nil.
-  split; first by set_solver.
-  split; first by set_solver.
-  split; first by assumption.
-  apply NoDup_app in Hlocks_held_NoDup.
-  intuition.
+  iSplit.
+  2: apply NoDup_app in Hlocks_held_NoDup; intuition.
+  iApply (is_slice_take_cap _ _ _ (word.sub acquired_s.(Slice.sz) 1)) in
+    "Hacquired_s".
+  1: rewrite fmap_length app_length /=; word.
+  replace (int.nat (word.sub _ 1)) with ((int.nat acquired_s.(Slice.sz)) - 1)%nat by word.
+  rewrite -fmap_take -Hacquired_s_sz Nat.add_sub take_app.
+  iFrame.
 Qed.
 
-Theorem wp_twophase__ReleaseAll (l: loc) locked_blknos γ dinit metamap:
+Lemma big_sepM_list_to_map `{Countable K} {A} l (Φ: K → A → iProp Σ) :
+  NoDup l.*1 →
+  ([∗ list] x ∈ l, Φ x.1 x.2) -∗
+  ([∗ map] k↦v ∈ list_to_map l, Φ k v).
+Proof.
+  induction l as [|x].
+  {
+    iIntros (HNoDup) "Hsep".
+    rewrite list_to_map_nil.
+    iApply big_sepM_empty.
+    auto.
+  }
+  iIntros (HNoDup) "Hsep".
+  destruct x as [k v].
+  rewrite list_to_map_cons.
+  iDestruct (big_sepL_cons with "Hsep") as "[Hx Hsep]".
+  rewrite fmap_cons in HNoDup.
+  apply NoDup_cons in HNoDup.
+  destruct HNoDup as [Hnotin HNoDup].
+  iApply big_sepM_insert.
+  {
+    apply not_elem_of_list_to_map_1.
+    auto.
+  }
+  simpl.
+  iFrame.
+  iApply ((IHl HNoDup) with "Hsep").
+Qed.
+
+Theorem wp_TwoPhase__ReleaseAll (l: loc) γ objs_dom locks_held :
   {{{
-    "Htwophase" ∷ is_twophase_inner l ∅ locked_blknos γ dinit metamap ∗
-    "Hlinvs" ∷ [∗ list] blkno ∈ locked_blknos, (
-      "Hlinv" ∷ linv γ metamap blkno
-    )
+    "Hlocks" ∷ is_twophase_locks l γ objs_dom locks_held ∗
+    "Hlinvs" ∷ ([∗ list] blkno ∈ locks_held, (
+      "Hlinv" ∷ twophase_linv γ objs_dom blkno
+    ))
   }}}
     TwoPhase__ReleaseAll #l
   {{{
-    RET #();
-    is_twophase_inner l ∅ [] γ dinit metamap
+    RET #(); True
   }}}.
 Proof.
   wp_start.
   wp_call.
   wp_apply (wp_forBreak_cond (λ b,
-    ∃ locked_blknos',
-      "Htwophase" ∷ is_twophase_inner l ∅ locked_blknos' γ dinit metamap ∗
-      "Hlinvs" ∷ ([∗ list] blkno ∈ locked_blknos', (
-        "Hlinv" ∷ linv γ metamap blkno
+    ∃ i,
+      "Hlocks" ∷ is_twophase_locks
+        l γ objs_dom (take i locks_held) ∗
+      "Hlinvs" ∷ ([∗ list] blkno ∈ take i locks_held, (
+        "Hlinv" ∷ twophase_linv γ objs_dom blkno
       )) ∗
-      "%Hb" ∷ ⌜b = false → locked_blknos' = []⌝
-  )%I with "[] [Htwophase Hlinvs]").
+      "%Hi" ∷ ⌜i ≤ length locks_held⌝ ∗
+      "%Hb" ∷ ⌜b = false → drop i locks_held = locks_held⌝
+  )%I with "[] [Hlocks Hlinvs]").
   2: {
-    iExists (locked_blknos).
+    iExists (length locks_held).
+    rewrite firstn_all drop_all.
     iFrame.
+    iSplit; first by auto.
     auto.
   }
   {
     iModIntro.
     iIntros (Φ') "Hloop HΦ'".
-    clear locked_blknos.
-    iDestruct "Hloop" as (locked_blknos) "(?&?&?)".
+    iDestruct "Hloop" as (i) "(?&?&?&?)".
     iNamed.
-    iNamed "Htwophase".
+    iNamed "Hlocks".
     wp_loadField.
     wp_apply wp_slice_len.
     iDestruct (is_slice_sz with "Hacquired_s") as "%Hlocked_blknos_len".
     wp_if_destruct.
     2: {
       iApply "HΦ'".
-      iExists locked_blknos.
+      iExists 0%nat.
       rewrite Heqb in Hlocked_blknos_len.
       replace (int.nat 0) with 0%nat in Hlocked_blknos_len by word.
       apply nil_length_inv in Hlocked_blknos_len.
-      subst locked_blknos.
-      iSplitL.
-      2: auto.
-      iExists _, _, _, _, _.
+      pose proof (take_drop i locks_held) as Htake_drop.
+      rewrite Hlocked_blknos_len app_nil_l in Htake_drop.
+      rewrite Hlocked_blknos_len take_0 drop_0.
+      iFrame.
+      iSplit.
+      2: {
+        iPureIntro.
+        split.
+        2: auto.
+        lia.
+      }
+      iExists _, _, _.
       iFrame "∗ #".
-      rewrite get_addr_map_blknos_nil list_to_set_nil.
       iPureIntro.
-      split; first by set_solver.
-      split; first by set_solver.
-      split; first by assumption.
       apply NoDup_nil_2.
     }
-    iAssert (is_twophase_inner l ∅ locked_blknos γ dinit metamap) with
-      "[Htwophase.buftxn Htwophase.locks Htwophase.acquired
-      Hbuftxn Hacquired_s Hlocked_blknos Hptstos]"
-    as "Htwophase".
+
+    iAssert (is_twophase_locks l γ objs_dom (take i locks_held))
+      with
+        "[Htwophase.locks Htwophase.acquired
+        Hacquired_s Hlocked_blknos]"
+      as "Htwophase".
     {
-      iExists _, _, _, _, _.
+      iExists _, _, _.
       iFrame "∗ # %".
     }
-    apply u64_val_ne in Heqb.
-    replace (int.Z 0) with 0 in Heqb by word.
-    assert (int.nat acquired_s.(Slice.sz) ≠ 0%nat) as Hacquired_s_sz by word.
-    rewrite -Hlocked_blknos_len in Hacquired_s_sz.
-    assert (0 < length locked_blknos)%nat as Hlocked_blknos by lia.
-    apply length_nonzero_neq_nil in Hlocked_blknos.
-    apply exists_last in Hlocked_blknos.
-    destruct Hlocked_blknos as (locked_blknos'&locked_tail&->).
+    destruct i.
+    {
+      rewrite take_0 /= in Hlocked_blknos_len.
+      apply u64_val_ne in Heqb.
+      replace (int.Z 0%Z) with 0%Z in Heqb by word.
+      word.
+    }
+    assert (i < length locks_held) as Hi_bounds by lia.
+    apply list_lookup_lt in Hi_bounds.
+    destruct Hi_bounds as [curr_lock Hcurr_lock].
+    rewrite (take_S_r _ _ _ Hcurr_lock).
     iDestruct (big_sepL_app with "Hlinvs") as "[Hlinvs Hlinv]".
     iDestruct (big_sepL_cons with "Hlinv") as "[? _]".
     iNamed.
-    wp_apply (wp_twophase__Release with "[$Htwophase $Hlinv]").
-    iIntros "Htwophase".
+    wp_apply (wp_TwoPhase__Release with "[$Htwophase $Hlinv]").
+    iNamed 1.
+
     wp_pures.
     iApply "HΦ'".
     iExists _.
     iFrame.
-    auto.
+    iPureIntro.
+    split; first by lia.
+    intros Hc.
+    inversion Hc.
   }
   iIntros "Hloop".
-  clear locked_blknos.
-  iDestruct "Hloop" as (locked_blknos) "(?&?&?)".
+  iDestruct "Hloop" as (?) "(?&?&?&?)".
   iNamed.
   pose proof (Hb eq_refl) as Hlocked_blknos.
-  subst.
+
   iApply "HΦ".
+  auto.
+Qed.
+
+Theorem wpc_TwoPhase__CommitNoRelease_raw {k} l γ γ' γtxn dinit objs_dom mt_committed mt_modified :
+  dom (gset addr) mt_committed = dom (gset addr) mt_modified →
+  {{{
+    "Htwophase" ∷ is_twophase_raw l γ γtxn dinit objs_dom mt_committed ∗
+    "Hbuftxn_mapstos" ∷ ([∗ map] a ↦ obj ∈ mt_modified,
+      "Hbuftxn_mapsto" ∷ buftxn_maps_to γtxn a obj
+    ) ∗
+    "#Htxn_cinv" ∷ txn_cinv Nbuftxn γ γ'
+  }}}
+    TwoPhase__CommitNoRelease #l @ S k; ⊤
+  {{{
+    (ok:bool) locks_held, RET #ok;
+    let locked_blknos: gset u64 := list_to_set locks_held in
+    let locked_addrs := filter_addr_set_by_blk locked_blknos objs_dom in
+    "Hlocks" ∷ is_twophase_locks l γ objs_dom locks_held ∗
+    "Htokens" ∷ (
+      [∗ set] a ∈ locked_addrs,
+        "Htoken" ∷ modify_token γ a
+    ) ∗
+    "Hdurable_mapstos" ∷ (
+      [∗ map] a ↦ obj ∈ (if ok then mt_modified else mt_committed),
+        "Hdurable_mapsto" ∷ durable_mapsto γ a obj
+    ) ∗
+    "%Hmt_dom" ∷ ⌜dom (gset addr) mt_committed ⊆ locked_addrs⌝
+  }}}
+  {{{
+    (
+      [∗ map] a ↦ obj ∈ mt_modified,
+        "Hdurable_mapsto" ∷ durable_mapsto γ' a obj
+    ) ∨ (
+      [∗ map] a ↦ obj ∈ mt_committed,
+        "Hdurable_mapsto" ∷ durable_mapsto γ' a obj
+    )
+  }}}.
+Proof.
+  remember (
+    [∗ map] a ↦ obj ∈ mt_committed, _
+  )%I as old_vals_durable.
+  remember (
+    [∗ map] a ↦ obj ∈ mt_modified, _
+  )%I as new_vals_durable.
+
+  iIntros (Hdom Φ Φc) "(?&?&?) HΦ".
+  iNamed.
+  iNamed "Htwophase".
+  iNamed "Hlocked_mapstos".
+  iNamed "Hbuftxn".
+  iApply wpc_cfupd.
+  rewrite /TwoPhase__CommitNoRelease.
+  wpc_pures.
+  {
+    iDestruct "HΦ" as "[HΦc _]".
+    iModIntro.
+    iMod (
+      exchange_durable_mapsto with "[$Htxn_cinv $Hlifted_mapstos]"
+    ) as "Hmapstos".
+    iModIntro.
+    iApply "HΦc".
+    iRight.
+    subst.
+    iApply (big_sepM_mono with "Hmapstos").
+    iIntros (a obj Hin) "(?&?)".
+    iFrame.
+  }
+  iCache (<disc> |C={⊤}_S k=> Φc)%I with "Hlifted_mapstos HΦ".
+  {
+    iDestruct "HΦ" as "[HΦc _]".
+    iModIntro.
+    iMod (
+      exchange_durable_mapsto with "[$Htxn_cinv $Hlifted_mapstos]"
+    ) as "Hmapstos".
+    iModIntro.
+    iApply "HΦc".
+    iRight.
+    subst.
+    iApply (big_sepM_mono with "Hmapstos").
+    iIntros (a obj Hin) "(?&?)".
+    iFrame.
+  }
+  wpc_frame_seq.
+  wp_apply util_proof.wp_DPrintf.
+  iNamed 1.
+  wpc_pures.
+  wpc_bind (struct.loadF _ _ _).
+  wpc_frame "HΦ Hlifted_mapstos".
+  wp_loadField.
+  iNamed 1.
+  wpc_apply (wpc_BufTxn__CommitWait' with "[
+    $Hbuftxn_mem Hbuftxn_durable_frag Hlifted_mapstos Hbuftxn_mapstos
+    Htxn_cinv
+  ]").
+  1-3: solve_ndisj.
+  1: subst; iFrame "∗ #".
+  iSplit.
+  {
+    iDestruct "HΦ" as "[HΦc _]".
+    iModIntro.
+    iIntros "Hmapstos".
+    iModIntro.
+    subst.
+    iDestruct "Hmapstos" as "[Hmapstos|Hmapstos]".
+    - iApply "HΦc".
+      iRight.
+      iApply (big_sepM_mono with "Hmapstos").
+      iIntros (a obj Hin) "(?&?)".
+      iFrame.
+    - iApply "HΦc".
+      iLeft.
+      iApply (big_sepM_mono with "Hmapstos").
+      iIntros (a obj Hin) "(?&?)".
+      iFrame.
+  }
+  iIntros (?) "!> Hmapstos".
+  iApply "HΦ".
+  iFrame (Hmt_dom) "Hlocks".
+  iDestruct (big_sepM_sep with "Hmapstos") as "[Htokens Hmapstos]".
+  iFrame "Hmapstos".
+  iDestruct (big_sepM_dom with "Htokens") as "Htokens".
+  remember (filter_addr_set_by_blk _ _) as locked_addrs.
+  replace ([∗ set] _ ∈ locked_addrs, _)%I with (
+    [∗ set] a ∈
+      locked_addrs ∖
+        dom (gset addr) mt_committed ∪
+        dom (gset addr) mt_committed,
+      modify_token γ a
+  )%I by (f_equal; rewrite difference_union_L; set_solver).
+  rewrite Hdom.
+  iApply (big_sepS_union with "[Hunlifted_mapstos Htokens]");
+    first by set_solver.
+  replace (dom _ (if ok then _ else _)) with (dom (gset addr) mt_modified);
+    last (destruct ok; rewrite ?Hdom //).
+  iFrame.
+Qed.
+
+Theorem wp_TwoPhase__readBufNoAcquire (l: loc) γ γtxn dinit objs_dom mt_committed a obj (sz: u64) :
+  is_Some (mt_committed !! a) →
+  bufSz (objKind obj) = int.nat sz →
+  {{{
+    "Htwophase" ∷ is_twophase_raw l γ γtxn dinit objs_dom mt_committed ∗
+    "Hmapsto" ∷ buftxn_maps_to γtxn a obj
+  }}}
+    TwoPhase__readBufNoAcquire #l (addr2val a) #sz
+  {{{
+    data_s data, RET (slice_val data_s);
+    "Htwophase" ∷ is_twophase_raw l γ γtxn dinit objs_dom mt_committed ∗
+    "Hmapsto" ∷ buftxn_maps_to γtxn a obj ∗
+    "Hdata_s" ∷ is_slice data_s byteT 1 data ∗
+    "%Hdata" ∷ ⌜data_has_obj data a obj⌝
+  }}}.
+Proof.
+  iIntros (Hlifted Hsz).
+  wp_start.
+  wp_call.
+  iNamed "Htwophase".
+  iNamed "Hbuftxn".
+  wp_loadField.
+  wp_apply (wp_BufTxn__ReadBuf with "[$Hbuftxn_mem $Hmapsto]");
+    first by assumption.
+  iIntros (??) "[Hbuf Hrestore]".
+  wp_apply (wp_buf_loadField_data with "Hbuf").
+  iIntros (?) "[Hbuf_data Hbuf_without_data]".
+  iDestruct (is_buf_data_has_obj with "Hbuf_data")
+    as (data) "[Hslice %Hdata]".
+  wp_apply (util_proof.wp_CloneByteSlice with "Hslice").
+  iIntros (s') "[Hslice Hclone]".
+  iDestruct (data_has_obj_to_buf_data with "Hslice") as "Hbuf_data";
+    first by eassumption.
+  iMod ("Hrestore" with "[Hbuf_data Hbuf_without_data] []")
+    as "[Hbuftxn_mem Hmapsto]";
+    [by (iExists _; iFrame)|by intuition|].
+  wp_pures.
+  iApply "HΦ".
+  iFrame (Hdata) "Hclone".
+  destruct obj.
+  simpl.
+  iFrame "Hmapsto".
+  iExists _.
+  iFrame (Hmt_dom) "Hlocks Hlocked_mapstos".
+  iExists _, _.
+  iFrame.
+Qed.
+
+Theorem wp_TwoPhase__ReadBuf_raw (l: loc) γ γtxn dinit objs_dom mt_committed a obj (sz: u64) :
+  a ∈ objs_dom →
+  bufSz (objKind obj) = int.nat sz →
+  {{{
+    "Htwophase" ∷ is_twophase_raw l γ γtxn dinit objs_dom mt_committed ∗
+    "Hmapsto" ∷ (
+      match mt_committed !! a with
+      | Some _ => buftxn_maps_to γtxn a obj
+      | None => durable_mapsto γ a obj
+      end
+    )
+  }}}
+    TwoPhase__ReadBuf #l (addr2val a) #sz
+  {{{
+    data_s data, RET (slice_val data_s);
+    let mt_committed' := (
+      match mt_committed !! a with
+      | Some _ => mt_committed
+      | None => <[a:=obj]>mt_committed
+      end
+    ) in
+    "Htwophase" ∷ is_twophase_raw l γ γtxn dinit objs_dom mt_committed' ∗
+    "Hmapsto" ∷ buftxn_maps_to γtxn a obj ∗
+    "Hdata_s" ∷ is_slice data_s byteT 1 data ∗
+    "%Hdata" ∷ ⌜data_has_obj data a obj⌝
+  }}}.
+Proof.
+  iIntros (Hwf Hsz).
+  wp_start.
+  wp_call.
+  wp_apply (wp_TwoPhase__Acquire_lift with "[$Htwophase $Hmapsto]");
+    first by assumption.
+  iNamed 1.
+  wp_apply (wp_TwoPhase__readBufNoAcquire with "[
+    $Htwophase $Hmapsto
+  ]"); [|assumption|].
+  {
+    destruct (mt_committed !! a) as [obj'|] eqn:Hlookup_old;
+      first by (rewrite Hlookup_old; eauto).
+    rewrite lookup_insert; eauto.
+  }
+  iIntros (??).
+  iNamed 1.
+  iApply "HΦ".
+  iFrame "∗ %".
+Qed.
+
+Theorem wp_TwoPhase__OverWrite_raw l γ γtxn dinit objs_dom mt_committed a (sz: u64) data_s data obj obj' :
+  bufSz (objKind obj') = int.nat sz →
+  data_has_obj data a obj' →
+  objKind obj' = objKind obj →
+  a ∈ objs_dom →
+  {{{
+    "Htwophase" ∷ is_twophase_raw l γ γtxn dinit objs_dom mt_committed ∗
+    "Hdata_s" ∷ is_slice_small data_s byteT 1 data ∗
+    "Hmapsto" ∷ (
+      match mt_committed !! a with
+      | Some _ => buftxn_maps_to γtxn a obj
+      | None => durable_mapsto γ a obj
+      end
+    )
+  }}}
+    TwoPhase__OverWrite #l (addr2val a) #sz (slice_val data_s)
+  {{{
+    RET #();
+    let mt_committed' := (
+      match mt_committed !! a with
+      | Some _ => mt_committed
+      | None => <[a:=obj]>mt_committed
+      end
+    ) in
+    "Htwophase" ∷ is_twophase_raw l γ γtxn dinit objs_dom mt_committed' ∗
+    "Hmapsto" ∷ buftxn_maps_to γtxn a obj'
+  }}}.
+Proof.
+  iIntros (Hsz Hdata Hkind Hwf).
+  wp_start.
+  wp_call.
+  wp_apply (wp_TwoPhase__Acquire_lift with "[$Htwophase $Hmapsto]");
+    first by assumption.
+  iNamed 1.
+  iNamed "Htwophase".
+  iNamed "Hbuftxn".
+  wp_loadField.
+  wp_apply (wp_BufTxn__OverWrite with "[$Hbuftxn_mem Hmapsto Hdata_s]").
+  1-3: by eassumption.
+  1: by iFrame.
+  iIntros "[Hbuftxn_mem Hmapsto]".
+
+  iApply "HΦ".
+  iFrame "Hmapsto".
+  iExists _.
+  iFrame (Hmt_dom) "Hlocks Hlocked_mapstos".
+  iExists _, _.
   iFrame.
 Qed.
